Write down GoLayer Layer definition

src/Goose/GoLayer.v
@@ -1,5 +1,14 @@
+From stdpp Require Import base.
+From RecordUpdate Require Import RecordUpdate.
+From Tactical Require Import ProofAutomation.
+
+From RecoveryRefinement Require Import Helpers.RelationAlgebra.
+
+From RecoveryRefinement Require Import Spec.Proc.
 From RecoveryRefinement Require Import Spec.InjectOp.
+From RecoveryRefinement Require Import Spec.Layer.
 From RecoveryRefinement Require Export Goose.Heap Goose.Filesys.
+
 
 Inductive Op : Type -> Type :=
 | FilesysOp : forall T, FS.Op T -> Op T
@@ -8,4 +17,38 @@ Inductive Op : Type -> Type :=
 Instance data_inj : Injectable Data.Op Op := DataOp.
 Instance fs_inj : Injectable FS.Op Op := FilesysOp.
 
-(* TODO: wrap up semantics and crash steps into a layer *)
+Module Go.
+  Notation State := FS.State.
+
+  Inductive step : forall T, Op T -> relation State State T :=
+  | StepFilesysOp T (op: FS.Op T) s res :
+      FS.step op s res ->
+      step (FilesysOp op) s res
+  | StepDataOpOk T (op: Data.Op T) s h' v :
+      Data.step op (FS.heap s) (Val h' v) ->
+      step (DataOp op) s (Val (set FS.heap (fun _ => h') s) v)
+  | StepDataOpErr T (op: Data.Op T) s :
+      Data.step op (FS.heap s) Err ->
+      step (DataOp op) s Err
+  .
+
+  Definition sem : Dynamics Op State :=
+    {| Proc.step := step;
+       Proc.crash_step := FS.crash_step;
+       Proc.finish_step := FS.crash_step; |}.
+
+  Definition l : Layer Op.
+    refine {| OpState := FS.State;
+              Layer.sem := sem;
+              trace_proj := fun _ => nil;
+              initP := fun s => s = ∅ |};
+      simpl; unfold puts;
+        propositional.
+    - auto.
+    - descend; intuition eauto.
+    - descend; intuition eauto.
+    - apply FS.crash_step_non_err in H; eauto.
+    - apply FS.crash_step_non_err in H; eauto.
+  Defined.
+
+End Go.
